Slight refactor

src/verification/semantics/skip_stream_multiply.lean
@@ -38,86 +38,66 @@ structure Stream.mul.ready {ι : Type} (a : Stream ι α) (b : Stream ι α) (s 
 local notation a ` ≺ `:50 b := Stream.wf_rel _ a b 
 
 @[simps]
-instance [has_mul α] : has_mul (Stream ι α) := ⟨λ (a b : Stream ι α),
+def Stream.mul [has_mul α] (a b : Stream ι α) : Stream ι α :=
 { σ := a.σ × b.σ,
   valid := λ p, a.valid p.1 ∧ b.valid p.2,
   ready := λ p, Stream.mul.ready a b p,
   skip := λ p hp i r, (a.skip p.1 hp.1 i r, b.skip p.2 hp.2 i r),
   index := λ p hv, max (a.index p.1 hv.1) (b.index p.2 hv.2),
-  value := λ p hr, a.value p.1 hr.r₁ * b.value p.2 hr.r₂,
-  wf_rel := prod.rprod_eq a.wf_rel b.wf_rel }⟩
+  value := λ p hr, a.value p.1 hr.r₁ * b.value p.2 hr.r₂ }
 
 section index_lemmas
 variables [has_mul α]
 
-lemma Stream.mul.ready.index' {a : Stream ι α} {b : Stream ι α} {x y} (h : (a * b).ready (x, y)) :
+lemma Stream.mul.ready.index' {a : Stream ι α} {b : Stream ι α} {x y} (h : (a.mul b).ready (x, y)) :
   a.index' x = b.index' y :=
 by simp [Stream.index'_val h.v₁, Stream.index'_val h.v₂, h.index]
 
-lemma Stream.mul.ready.order_eq {a : Stream ι α} {b : Stream ι α} {x y} (h : (a * b).ready (x, y)) :
+lemma Stream.mul.ready.order_eq {a : Stream ι α} {b : Stream ι α} {x y} (h : (a.mul b).ready (x, y)) :
   a.to_order x = b.to_order y :=
 by ext : 1; simp [h.r₁, h.r₂, h.index']
 
 lemma Stream.mul_index' (a b : Stream ι α) (xy : a.σ × b.σ) :
-  (a * b).index' xy = max (a.index' xy.1) (b.index' xy.2) :=
+  (a.mul b).index' xy = max (a.index' xy.1) (b.index' xy.2) :=
 begin
   cases xy with x y,
   rw [Stream.index'],
-  simp only [Stream.has_mul_mul_index, with_top.coe_max],
+  simp only [Stream.mul_index, with_top.coe_max],
   split_ifs with h,
   { simp [Stream.index'_val h.1, Stream.index'_val h.2], },
   erw not_and_distrib at h, cases h; simp [h],
 end
 
 /-- This lemma takes a surprising amount of effort to prove -/
-lemma Stream.min_to_order_le (a b : Stream ι α) (q : a.σ × b.σ) (hv : (a * b).valid q) :
-  min (a.to_order q.1) (b.to_order q.2) ≤ (a * b).to_order q :=
+lemma Stream.min_to_order_le (a b : Stream ι α) (q : a.σ × b.σ) (hv : (a.mul b).valid q) :
+  min (a.to_order q.1) (b.to_order q.2) ≤ (a.mul b).to_order q :=
 begin
   rw prod.lex.le_iff'', 
   simp only [monotone.map_min (@prod.lex.fst_mono (with_top ι) bool _ _)],
   split, { convert min_le_max, simp [Stream.mul_index'], },
   intro h,
   replace h : a.index' q.1 = b.index' q.2 := by simpa [Stream.mul_index'] using h,
-  suffices : a.ready q.1 → b.ready q.2 → (a * b).ready q,
+  suffices : a.ready q.1 → b.ready q.2 → (a.mul b).ready q,
   { simpa [Stream.to_order, h, prod.lex.mk_min, bool.min_eq_and, bool.le_iff_imp], },
   intros hr₁ hr₂,
   refine ⟨hv.1, hv.2, hr₁, hr₂, _⟩,
   simpa [hv.1, hv.2] using h,
 end
 
-end index_lemmas
+lemma mul_rel_wf (a b : BoundedStream ι α) : well_founded (prod.rprod_eq a.wf_rel b.wf_rel) :=
+prod.rprod_eq_wf a.wf b.wf
 
-variables [non_unital_non_assoc_semiring α]
-
-@[simp]
-def LawfulStream.mul (a b : LawfulStream ι α) : Stream ι α := a.to_Stream * b.to_Stream
-
-namespace LawfulStream.mul
-open Stream
-
-variables {a b : LawfulStream ι α}
-
-lemma mul_is_skip_valid : skip_valid_wf (a.mul b) :=
+lemma mul_is_skip_valid {a b : BoundedStream ι α} (ha : a.skip_valid_wf a.wf_rel) (hb : b.skip_valid_wf b.wf_rel) :
+  (a.mul b.to_Stream).skip_valid_wf (prod.rprod_eq a.wf_rel b.wf_rel) :=
 begin
-  split, { refine prod.rprod_eq_wf a.skip_wf.wf b.skip_wf.wf, },
   intros q hq i r,
-  rcases a.skip_wf.no_backward q.1 hq.1 i r with (h|⟨ha₁, ha₂⟩),
-  { exact or.inl (or.inl ⟨h, b.skip_wf.no_backward' _ _ _ _⟩), },
-  rcases b.skip_wf.no_backward q.2 hq.2 i r with (h|⟨hb₁, hb₂⟩),
-  { exact or.inl (or.inr ⟨h, a.skip_wf.no_backward' _ _ _ _⟩), },
+  rcases ha q.1 hq.1 i r with (h|⟨ha₁, ha₂⟩),
+  { exact or.inl (or.inl ⟨h, hb.no_backward _ _ _ _⟩), },
+  rcases hb q.2 hq.2 i r with (h|⟨hb₁, hb₂⟩),
+  { exact or.inl (or.inr ⟨h, ha.no_backward _ _ _ _⟩), },
   right, split, swap,
   { dsimp, simp [ha₂, hb₂], },
   exact lt_of_lt_of_le (lt_min ha₁ hb₁) (Stream.min_to_order_le _ _ _ hq),
 end
 
--- lemma rel_iff  (q₁ q₂ : a.σ × b.σ) :
---   (q₁ ≺ₘ q₂) ↔ (q₁.1 ≺ q₂.1) ∧ (q₁.2 ≺ q₂.2) := by rw [rel, prod.rprod_iff]
-
--- lemma rel_wf : well_founded (@rel _ _ _ _ a b) := prod.rprod_wf a.rel_wf b.rel_wf
-
-
-
-end LawfulStream.mul
-
--- theorem LawfulStream.mul_spec (s₁ s₂ : LawfulStream ι α) (q₁ : s₁.σ) (q₂ : s₂.σ) :
---   (s₁.mul s₂).eval 
+end index_lemmas
